---
{"dg-publish":true,"dg-path":"CIS/Discrete Structures/Summation Notation.md","permalink":"/cis/discrete-structures/summation-notation/","created":"2024-03-27T16:06:09.433-04:00","updated":"2025-07-08T10:47:55.444-04:00"}
---

$$
\sum_{i=m}^nx_{i}=x_{m}+x_{m+1}+\dots+x_{n-1}+x_{n}
$$
$$
\sum_{i=0}^n xi = x \sum_{i=0}^n i
$$
$$
\sum x \pm \sum y = \sum x \pm y 
$$
$$
\sum_{i=m}^n x_{i} = \sum_{i=m+k}^{n+k}(x_{i-k})
$$
$$
\sum_{x=1}^n(n-x)=\sum_{x=1}^{n-1}x
$$
$$
\begin{align}
\sum_{i=1}^n(n-i)  & =\sum n-\sum i \\
 & =n\cdot n- \frac{n(n+1)}{2} &  \\
 & =n^2- \frac{n^2+n}{2} \\
 & =\frac{2n^2-(n^2+n)}{2} \\
 & =\frac{n^2-n}{2} \\
 & =\frac{n(n-1)}{2} \\
 \sum_{x=1}^n(n-x) & = \sum_{x=1}^{n-1}x\neq \sum_{x=1}^nx
\end{align}
$$
$$\begin{align}
\sum_{i=0}^n n-i & = (n+1)n - \frac{n(n+1)}{2} \\
 & =\frac{2n(n+1)-n(n+1)}{2} \\
 & =\frac{n(n+1)}{2}
\end{align} 
$$
$$
\sum_{x=1}^n(n-x)=n-n+\sum_{x=1}^{n-1}(n-x)=\sum_{x=1}^{n-1}(n-x)
$$
$$
\sum_{i=1}^n i^2 = \frac{n\cdot(n+1)\cdot(2n+1)}{6}
$$
$$
\sum_{i=1}^n i^3 = \left( \sum_{i=1}^ni \right)^2 = \left( \frac{n(n+1)}{2} \right)^2
$$
$$
\sum_{i=0}^n a^i = \frac{a^{n+1}-1}{a-1}
$$
